nola/iris/cif.v
@@ -2,11 +2,35 @@
 
 From nola.util Require Export uip (** Assume UIP over any type *).
 From nola.util Require Export nary cit.
+From nola.bi Require Export deriv.
 From nola.bi Require Import later.
 From nola.iris Require Export iprop.
-Import iPropAppNotation FunPRNotation.
+Import EqNotations iPropAppNotation FunPRNotation DsemNotation.
 
-(** ** Data types *)
+(** ** [cifcon]: Custom constructor structure for [cif] *)
+#[projections(primitive)]
+Structure cifcon := Cifcon {
+  (** Selector of custom constructors *) cifc_sel :> Type;
+  (** Domain for inductive parts *) #[canonical=no] cifc_idom : cifc_sel → Type;
+  (** Domain for coinductive parts *) #[canonical=no]
+    cifc_cdom : cifc_sel → Type;
+  (** Data [oFunctor] *) #[canonical=no] cifc_data : cifc_sel → oFunctor;
+  (** [cifc_data] is contractive *) #[canonical=no]
+    cifc_data_contractive {s} :: oFunctorContractive (cifc_data s);
+}.
+Add Printing Constructor cifcon.
+Arguments cifc_sel CON : rename. Arguments cifc_idom CON : rename.
+Arguments cifc_cdom CON : rename. Arguments cifc_data CON : rename.
+Arguments cifc_data_contractive CON {_} : rename.
+Implicit Type CON : cifcon.
+
+(** Big sum of [cifcon]s *)
+Canonical sigTCC {A} (CONF : A → cifcon) := Cifcon (sigT CONF)
+  (λ ss, (CONF _).(cifc_idom) (projT2 ss))
+  (λ ss, (CONF _).(cifc_cdom) (projT2 ss))
+  (λ ss, (CONF _).(cifc_data) (projT2 ss)) _.
+
+(** ** Data types for [cif] *)
 
 (** [cif_binsel]: Binary operator selector *)
 Variant cif_binsel :=
@@ -24,75 +48,74 @@ Variant cif_unsel :=
 | (** Except-0 *) cifs_except0.
 
 (** [cif_sel]: Selector *)
-Variant cif_sel SEL :=
+Variant cif_sel CON :=
 | (** Universal quantifier *) cifs_all (A : Type)
 | (** Existential quantifier *) cifs_ex (A : Type)
 | (** Binary operator *) cifs_bin (s : cif_binsel)
 | (** Unary operator *) cifs_un (s : cif_unsel)
 | (** Pure proposition *) cifs_pure
 | (** Later *) cifs_later
-| (** Custom selector *) cifs_custom (s : SEL).
+| (** Custom selector *) cifs_custom (s : CON).
 Arguments cifs_all {_}. Arguments cifs_ex {_}.
 Arguments cifs_bin {_}.  Arguments cifs_un {_}.
 Arguments cifs_pure {_}. Arguments cifs_later {_}. Arguments cifs_custom {_}.
 
 (** [cif_idom]: Domain for inductive parts *)
-Definition cif_idom {SEL} (I : SEL → Type) (s : cif_sel SEL) : Type :=
+Definition cif_idom CON (s : cif_sel CON) : Type :=
   match s with
   | cifs_all A | cifs_ex A => A | cifs_bin _ => bool | cifs_un _ => unit
-  | cifs_pure | cifs_later => Empty_set | cifs_custom s => I s
+  | cifs_pure | cifs_later => Empty_set | cifs_custom s => CON.(cifc_idom) s
   end.
 
 (** [cif_cdom]: Domain for coinductive parts *)
-Definition cif_cdom {SEL} (C : SEL → Type) (s : cif_sel SEL) : Type :=
+Definition cif_cdom CON (s : cif_sel CON) : Type :=
   match s with
   | cifs_all _ | cifs_ex _ | cifs_bin _ | cifs_un _ | cifs_pure | cifs_later =>
       Empty_set
-  | cifs_custom s => C s
+  | cifs_custom s => CON.(cifc_cdom) s
   end.
 
-(** [cif_dataOF]: Data [oFunctor] *)
-Definition cif_dataOF {SEL} (D : SEL → oFunctor) (s : cif_sel SEL) : oFunctor :=
+(** [cif_data]: Data [oFunctor] *)
+Definition cif_data CON (s : cif_sel CON) : oFunctor :=
   match s with
   | cifs_all _ | cifs_ex _ | cifs_bin _ | cifs_un _ => unitO
-  | cifs_pure => PropO | cifs_later => laterOF ∙ | cifs_custom s => D s
+  | cifs_pure => PropO | cifs_later => laterOF ∙
+  | cifs_custom s => CON.(cifc_data) s
   end.
 
-(** [cif_dataOF] is contractive *)
-#[export] Instance cif_dataOF_contractive {SEL s}
-  `{∀ s : SEL, oFunctorContractive (D s)} :
-  oFunctorContractive (cif_dataOF D s).
+(** [cif_data] is contractive *)
+#[export] Instance cif_data_contractive {CON s} :
+  oFunctorContractive (cif_data CON s).
 Proof. case s=>/=; exact _. Qed.
 
 (** ** [cif]: Coinductive-inductive set of formulas *)
-Definition cifOF {SEL} I C D : oFunctor :=
-  citOF (cif_idom (SEL:=SEL) I) (cif_cdom C) (cif_dataOF D).
-Definition cifPR {SEL} I C D Σ : prost :=
-  citPR (cif_idom (SEL:=SEL) I) (cif_cdom C) (λ s, cif_dataOF D s $oi Σ).
-Definition cifO {SEL} I C D Σ : ofe := @cifPR SEL I C D Σ.
-Definition cif {SEL} I C D Σ : Type := @cifPR SEL I C D Σ.
-Definition cifaPR {SEL} I C D Σ : prost :=
-  citaPR (cif_idom (SEL:=SEL) I) (cif_cdom C) (λ s, cif_dataOF D s $oi Σ).
-Definition cifaO {SEL} I C D Σ : ofe := @cifaPR SEL I C D Σ.
-Definition cifa {SEL} I C D Σ : Type := @cifaPR SEL I C D Σ.
+Definition cifOF CON : oFunctor :=
+  citOF (cif_idom CON) (cif_cdom CON) (cif_data CON).
+Definition cifPR CON Σ : prost :=
+  citPR (cif_idom CON) (cif_cdom CON) (λ s, cif_data CON s $oi Σ).
+Definition cifO CON Σ : ofe := cifPR CON Σ.
+Definition cif CON Σ : Type := cifPR CON Σ.
+Definition cifaPR CON Σ : prost :=
+  citaPR (cif_idom CON) (cif_cdom CON) (λ s, cif_data CON s $oi Σ).
+Definition cifaO CON Σ : ofe := cifaPR CON Σ.
+Definition cifa CON Σ : Type := cifaPR CON Σ.
 
 (** [cifOF] is contractive *)
-#[export] Instance cifOF_contractive {SEL I C}
-  `{∀ s, oFunctorContractive (D s)} : oFunctorContractive (@cifOF SEL I C D).
+#[export] Instance cifOF_contractive {CON} : oFunctorContractive (cifOF CON).
 Proof. exact _. Qed.
 
 (** ** Construct [cif] *)
 Section cif.
-  Context {SEL} {I C : SEL → Type} {D : SEL → oFunctor} {Σ : gFunctors}.
+  Context {CON} {Σ : gFunctors}.
 
   (** Basic connectives *)
 
-  Definition cif_all {A} (Φx : A -pr> cif I C D Σ) : cif I C D Σ :=
+  Definition cif_all {A} (Φx : A -pr> cif CON Σ) : cif CON Σ :=
     Citg (cifs_all A) Φx nullary ().
-  Definition cif_ex {A} (Φx : A -pr> cif I C D Σ) : cif I C D Σ :=
+  Definition cif_ex {A} (Φx : A -pr> cif CON Σ) : cif CON Σ :=
     Citg (cifs_ex A) Φx nullary ().
 
-  Definition cif_bin (s : cif_binsel) (Px Qx : cif I C D Σ) : cif I C D Σ :=
+  Definition cif_bin (s : cif_binsel) (Px Qx : cif CON Σ) : cif CON Σ :=
     Citg (cifs_bin s) (binary Px Qx) nullary ().
   Definition cif_and := cif_bin cifs_and.
   Definition cif_or := cif_bin cifs_or.
@@ -100,25 +123,26 @@ Section cif.
   Definition cif_sep := cif_bin cifs_sep.
   Definition cif_wand := cif_bin cifs_wand.
 
-  Definition cif_un (s : cif_unsel) (Px : cif I C D Σ) : cif I C D Σ :=
+  Definition cif_un (s : cif_unsel) (Px : cif CON Σ) : cif CON Σ :=
     Citg (cifs_un s) (unary Px) nullary ().
   Definition cif_plain := cif_un cifs_plain.
   Definition cif_pers := cif_un cifs_pers.
   Definition cif_bupd := cif_un cifs_bupd.
   Definition cif_except0 := cif_un cifs_except0.
 
-  Definition cif_pure (φ : Prop) : cif I C D Σ :=
+  Definition cif_pure (φ : Prop) : cif CON Σ :=
     Citg cifs_pure nullary nullary φ.
-  Definition cif_later (P : iProp Σ) : cif I C D Σ :=
+  Definition cif_later (P : iProp Σ) : cif CON Σ :=
     Citg cifs_later nullary nullary (Next P%I).
 
   (** Custom connective *)
-  Definition cif_custom s (Φx : I s -pr> cif I C D Σ)
-    (Ψx : C s -pr> cif I C D Σ) (d : D s $oi Σ) : cif I C D Σ :=
+  Definition cif_custom (s : CON) (Φx : CON.(cifc_idom) s -pr> cif CON Σ)
+    (Ψx : CON.(cifc_cdom) s -pr> cif CON Σ) (d : CON.(cifc_data) s $oi Σ)
+    : cif CON Σ :=
     Citg (cifs_custom s) Φx (λ c, of_cit (Ψx c)) d.
 
   (** [cif] is inhabited *)
-  #[export] Instance cif_inhabited : Inhabited (cif I C D Σ) :=
+  #[export] Instance cif_inhabited : Inhabited (cif CON Σ) :=
     populate (cif_pure True).
 
   (** Basic connectives are size-preserving *)
@@ -212,16 +236,29 @@ Notation "'True'" := (cif_pure True) : cif_scope.
 Notation "'False'" := (cif_pure False) : cif_scope.
 Notation "▷ P" := (cif_later P) : cif_scope.
 
+Implicit Type JUDG : ofe.
+
+(** ** Semantics for [cifcon] *)
+#[projections(primitive)]
+Record SemCifcon (JUDG : ofe) CON Σ := SEM_CIFCON {
+  (** Semantics *)
+  sem_cifc :> (JUDG → iProp Σ) → ∀ s, (CON.(cifc_idom) s -d> iProp Σ) →
+    (CON.(cifc_cdom) s -d> cif CON Σ) → CON.(cifc_data) s $oi Σ → iProp Σ;
+  (** [sem_cifc] is non-expansive *)
+  sem_cifc_ne `{!NonExpansive δ} {s} :: NonExpansive3 (sem_cifc δ s);
+}.
+Existing Class SemCifcon.
+Arguments SEM_CIFCON {_ _ _} _ _. Arguments sem_cifc {_ _ _ semc} : rename.
+Arguments sem_cifc_ne {_ _ _ semc _ _ _} : rename.
+
 (** ** [cif_sem]: Semantics of [cif] *)
 Section iris.
-  Context {SEL} {I C : SEL → Type} {D : SEL → oFunctor} {Σ : gFunctors}.
+  Context `{!SemCifcon JUDG CON Σ}.
 
   (** [cif_bsem]: Base semantics for [cif] *)
-  Definition cif_bsem
-    (sm : ∀ s, (I s -d> iProp Σ) → (C s -d> cif I C D Σ) →
-      D s $oi Σ → iProp Σ) s
-    : (cif_idom I s -d> iProp Σ) → (cif_cdom C s -d> cif I C D Σ) →
-        cif_dataOF D s $oi Σ → iProp Σ :=
+  Definition cif_bsem δ s :
+    (cif_idom CON s -d> iProp Σ) → (cif_cdom CON s -d> cif CON Σ) →
+        cif_data CON s $oi Σ → iProp Σ :=
     match s with
     | cifs_all _ => λ Φ _ _, ∀ a, Φ a | cifs_ex _ => λ Φ _ _, ∃ a, Φ a
     | cifs_bin s => λ Φ _ _, let P := Φ true in let Q := Φ false in
@@ -235,30 +272,89 @@ Section iris.
         | cifs_except0 => ◇ P
         end
     | cifs_pure => λ _ _ φ, ⌜φ⌝ | cifs_later => λ _ _, laterl
-    | cifs_custom s => sm s
+    | cifs_custom s => sem_cifc δ s
     end%I.
 
   (** [cif_bsem] is non-expansive *)
-  #[export] Instance cif_bsem_ne `{!∀ s, NonExpansive3 (sm s)} {s} :
-    NonExpansive3 (cif_bsem sm s).
-  Proof.
-    case s=>/=; try solve_proper. move=> ???????. by apply laterl_ne.
-  Qed.
+  #[export] Instance cif_bsem_ne `{!NonExpansive δ} {s} :
+    NonExpansive3 (cif_bsem δ s).
+  Proof. case s=>/=; try solve_proper. move=> ???????. by apply laterl_ne. Qed.
 End iris.
 
 (** [cif_sem]: Semantics of [cif] *)
-Notation cif_sem sm := (cit_fold (cif_bsem sm)).
-Notation cif_sem' SEL I C D Σ sm := (cit_fold (@cif_bsem SEL I C D Σ sm))
-  (only parsing).
+Notation cif_sem δ := (cit_fold (cif_bsem δ)).
 
 Section iris.
-  Context {SEL} {I C : SEL → Type} {D : SEL → oFunctor} {Σ : gFunctors}.
+  Context `{!SemCifcon JUDG CON Σ}.
 
-  (** [cif_sem sm] is non-expansive if [sm] is *)
-  #[export] Instance cif_sem_ne `{!∀ s, NonExpansive3 (sm s)} :
-    NonExpansive (cif_sem' _ I C D Σ sm).
+  (** [cif_sem] is non-expansive *)
+  #[export] Instance cif_sem_ne `{!NonExpansive δ} : NonExpansive (cif_sem δ).
   Proof. move=> ?. apply cit_fold_ne_gen; solve_proper. Qed.
-  #[export] Instance cif_sem_proper `{!∀ s, NonExpansive3 (sm s)} :
-    Proper ((≡) ==> (⊣⊢)) (cif_sem' _ I C D Σ sm).
+  #[export] Instance cif_sem_proper `{!NonExpansive δ} :
+    Proper ((≡) ==> (≡)) (cif_sem δ).
   Proof. apply ne_proper, _. Qed.
+  (** [Dsem] over [cif] *)
+  #[export] Instance cif_dsem : Dsem JUDG (cifO CON Σ) (iProp Σ) :=
+    DSEM (λ δ, cif_sem δ) _.
 End iris.
+
+(** ** Element [cifcon] *)
+
+(** [Ecifcon]: Element [cifcon] *)
+#[projections(primitive)]
+Class Ecifcon CON' CON := ECIFCON {
+  ecifc_sel : CON' → CON;
+  ecifc_idom {s} : CON.(cifc_idom) (ecifc_sel s) = CON'.(cifc_idom) s;
+  ecifc_cdom {s} : CON.(cifc_cdom) (ecifc_sel s) = CON'.(cifc_cdom) s;
+  ecifc_data {s} : CON.(cifc_data) (ecifc_sel s) = CON'.(cifc_data) s;
+}.
+Arguments ECIFCON {_ _}.
+
+(** Inclusion into [sigTCC] *)
+#[export] Instance sigT_ecifcon {A CONF a} :
+  Ecifcon (CONF a) (@sigTCC A CONF) :=
+  ECIFCON (existT a) (λ _, eq_refl) (λ _, eq_refl) (λ _, eq_refl).
+
+(** Custom constructor under [Ecifcon] *)
+Program Definition cif_ecustom `{!Ecifcon CON' CON} {Σ} (s : CON')
+  (Φx : CON'.(cifc_idom) s -pr> cif CON Σ)
+  (Ψx : CON'.(cifc_cdom) s -pr> cif CON Σ) (d : CON'.(cifc_data) s $oi Σ)
+  : cif CON Σ :=
+  cif_custom (ecifc_sel s) (λ i, Φx (rew[id] ecifc_idom in i))
+    (λ c, Ψx (rew[id] ecifc_cdom in c))
+    (rew[λ F, F $oi Σ] eq_sym ecifc_data in d).
+
+(** Semantics of an element [cifcon] *)
+#[projections(primitive)]
+Record SemEcifcon JUDG CON' CON Σ := SEM_ECIFCON {
+  (** Semantics *)
+  sem_ecifc :> (JUDG → iProp Σ) → ∀ s, (CON'.(cifc_idom) s -d> iProp Σ) →
+    (CON'.(cifc_cdom) s -d> cif CON Σ) → CON'.(cifc_data) s $oi Σ → iProp Σ;
+  (** [sem_ecifc] is non-expansive *)
+  sem_ecifc_ne `{!NonExpansive δ} {s} :: NonExpansive3 (sem_ecifc δ s);
+}.
+Existing Class SemEcifcon.
+Arguments SEM_ECIFCON {_ _ _ _} _ _.
+Arguments sem_ecifc {_ _ _ _ semec} : rename.
+Arguments sem_ecifc_ne {_ _ _ _ semec _ _ _} : rename.
+
+(** [SemCifcon] over [sigT] by [SemEcifcon] *)
+#[export] Program Instance sigT_sem_cifcon {JUDG A}
+  `{semec : !∀ a, SemEcifcon JUDG (CONF a) (@sigTCC A CONF) Σ}
+  : SemCifcon JUDG (sigTCC CONF) Σ :=
+  SEM_CIFCON (λ δ s, semec _ δ (projT2 s)) _.
+Next Obligation. solve_proper. Qed.
+
+(** Inclusion with respect to [SemEcifcon] and [SemCifcon] *)
+Class EsemEcifcon JUDG CON' CON Σ `{!Ecifcon CON' CON}
+  `{!SemEcifcon JUDG CON' CON Σ, !SemCifcon JUDG CON Σ} :=
+  esem_ecifc : ∀ {δ s Φ Ψx d},
+    sem_cifc δ (ecifc_sel s) (λ i, Φ (rew[id] ecifc_idom in i))
+      (λ c, Ψx (rew[id] ecifc_cdom in c))
+      (rew[λ F, F $oi Σ] eq_sym ecifc_data in d) =
+      sem_ecifc δ s Φ Ψx d.
+
+(** [EsemEcifcon] into [sigT] *)
+#[export] Instance sigT_esem_cifcon {JUDG A}
+  `{semec : !∀ a, SemEcifcon JUDG (CONF a) (@sigTCC A CONF) Σ} {a} :
+  EsemEcifcon JUDG (CONF a) (sigTCC CONF) Σ := λ _ _ _ _ _, eq_refl.
